Rewriting shadow memory to add support for values.

src/Memory.v
@@ -1,119 +1,138 @@
+Set Implicit Arguments.
+
+Require Import Coq.Lists.List.
 Require Import Tid.
 Require Import Lang.
-Require Import Dep.
 Require Import Mid.
+Require Import Shadow.
+Require Import Node.
+
+Module Locals.
+Section Defs.
+  Variable A:Type.
+
+  Inductive op :=
+  | CONS : A -> node -> op
+  | NEW : list A -> op.
+
+  Definition task_local := list A.
+
+  Definition local_memory := MN.t task_local.
+
+  Inductive Reduces (m:local_memory): (node * op) -> local_memory -> Prop :=
+  | reduces_add:
+    forall l x n n',
+    MN.MapsTo n l m ->
+    ~ MN.In n' m ->
+    Reduces m (n', CONS x n) (MN.add n' (x::l) m)
+  | reduces_new:
+    forall l n,
+    ~ MN.In n m ->
+    Reduces m (n, NEW l) (MN.add n l m).
+
+  Inductive MapsTo (n:node) (x:A) (ls:local_memory) : Prop :=
+  | local_def:
+    forall l,
+    MN.MapsTo n l ls ->
+    List.In x l ->
+    MapsTo n x ls.
+
+End Defs.
+End Locals.
 
 Section Defs.
-  Definition local := list (tid * dep). (*MT.t (list dep).*)
-  Definition global := MM.t (option dep).
 
-  Definition memory := (global * local) % type.
+  Import Locals.
+
+  Inductive datum :=
+  | d_task : tid -> datum
+  | d_mem : mid -> datum
+  | d_any : datum.
+
+
+  Definition global_memory := access_history datum.
+
+  Definition memory := (global_memory * (local_memory datum)) % type.
 
   Definition m_global (m:memory) := fst m.
 
   Definition m_local (m:memory) := snd m.
 
   Inductive op :=
-(*  | LOCAL_REM: dep -> op*)
-  | GLOBAL_CREATE: mid -> option dep -> op
-  | GLOBAL_PUT: mid -> option dep -> op
-  | GLOBAL_GET: mid -> op
-  | FUTURE: tid -> list dep -> op
-  | FORCE: tid -> list dep -> op.
-(*
-  Definition local_update f (t:tid) (l:local) : local :=
-  match MT.find t l with
-  | Some ds => MT.add t (f ds)%list l
-  | _ => l
-  end.
-*)
-  Notation local_entry := (tid * dep) % type.
+  | CONTINUE: op
+  | GLOBAL_ALLOC: mid -> datum -> op
+  | GLOBAL_WRITE: mid -> datum -> op
+  | GLOBAL_READ: mid -> op
+  | FUTURE: node -> list datum -> op
+  | FORCE: node -> datum -> op.
 
-  Definition local_add t d (l:local) : local := cons (t,d) l. (*local_update (cons d) % list t.*)
+  Definition effect := (node * node * op) % type.
 
-  Fixpoint local_add_all t ds (l:local) : local :=
-  match ds with
-  | cons d ds => local_add t d (local_add_all t ds l)
-  | nil => l
-  end.
+  Require Import CG.
 
-  Let local_entry_eq_dec :
-    forall (x y : local_entry),
-    { x = y } + { x <> y }.
-  Proof.
-    intros.
-    destruct x as (x1,x2), y as (y1, y2).
-    destruct (tid_eq_dec x1 y1), (dep_eq_dec x2 y2);
-    subst;
-    auto;
-    right;
-    intuition;
-    inversion H;
-    subst;
-    contradiction n;
-    auto.
-  Qed.
-
-  Definition local_remove (t:tid) (d:dep) (l:local) := List.remove local_entry_eq_dec (t,d) l. (*local_update (List.remove dep_eq_dec d) t.*)
-
-(*  Definition local_create (t:tid) (ds:list dep) (l:local) : local := MT.add t ds l.*)
-
-  Definition effect := (tid * op) % type.
-
-  Inductive In (t:tid) (l:local) : Prop :=
-  | in_def:
-    forall d,
-    List.In (t, d) l ->
-    In t l.
-
-  Inductive Local (l:local) x (d:dep) : Prop :=
-  | local_def:
-    List.In (x,d) l ->
-    Local l x d.
+  Variable cg: computation_graph.
 
   Inductive Reduces : memory -> effect -> memory -> Prop :=
-  | reduces_g_get: (* read *)
-    forall g l x t d,
-    Local l t (d_mid x) ->
-    MM.MapsTo x (Some d) g ->
-    Reduces (g, l) (t, GLOBAL_GET x) (g, local_add t d l)
-  | reduces_g_put: (* write *)
-    forall g l x t o,
-    Local l t (d_mid x) ->
-    Reduces (g, l) (t, GLOBAL_PUT x o) (MM.add x o g, l)
-(*  | reduces_l_rem: (* local store of a constant *)
-    forall l g t o,
-    In t l ->
-    Reduces (g, l) (t, LOCAL_REM o) (g, local_remove t o l)*)
-  | reduces_g_create: (* malloc *)
-    forall g l x t o,
-    ~ MM.In x g ->
-    Local l t (d_mid x) ->
-    Reduces (g, l) (t, GLOBAL_CREATE x o) (MM.add x o g, l)
-  | reduces_future: (* future *)
-    forall t t' ds l g,
-    List.Forall (Local l t) ds ->
-    ~ In t' l ->
-    Reduces (g, l) (t, FUTURE t' ds) (g, local_add_all t' ds (local_add t (d_tid t') l))
-  | reduce_force: (* force *)
-    forall g l t t' d ds,
-    List.Forall (Local l t) ds ->
-    Reduces (g, l) (t, FORCE t' ds) (g, local_add t d l).
+  | reduces_g_read:
+    forall g l d n n' x l' g',
+    Locals.MapsTo n (d_mem x) l ->
+    Shadow.MapsTo x d g cg ->
+    Locals.Reduces l (n', CONS d n) l' ->
+    Shadow.Reduces cg g (x, {| a_when := n; a_what:=@READ datum |}) g' ->
+    Reduces (g, l) (x, GLOBAL_READ x) (g', l')
+
+  | reduces_g_write:
+    forall g (l:local_memory datum) x d n n' g',
+    Locals.MapsTo n d l ->
+    Locals.MapsTo n (d_mem x) l ->
+    Shadow.Reduces cg g (x, {| a_when:=n; a_what:=WRITE d|}) g' ->
+    Reduces (g, l) (n, n', GLOBAL_WRITE x d) (g', l)
+
+  | reduces_g_alloc:
+    forall g l x n n' d l' g',
+    Locals.MapsTo n d l ->
+    Shadow.Reduces cg g (x, {|a_when:=n;a_what:=ALLOC d|}) g' ->
+    Locals.Reduces l (n', CONS (d_mem x) n) l' ->
+    Reduces (g, l) (n, n', GLOBAL_ALLOC x d) (g', l')
+
+  | reduces_future:
+    forall nx nx' ny ds l g y l' l'',
+    List.Forall (fun d => Locals.MapsTo nx d l) ds ->
+    Node.MapsTo y ny (fst cg) ->
+    Locals.Reduces l (nx', CONS (d_task y) nx) l' ->
+    Locals.Reduces l' (ny, NEW ds) l'' ->
+    Reduces (g, l) (nx, nx', FUTURE ny ds) (g, l)
+
+  | reduce_force:
+    forall g l nx nx' ny d l',
+    Locals.MapsTo ny d l ->
+    Locals.Reduces l (nx, CONS d nx') l' ->
+    Reduces (g, l) (nx, nx', FORCE ny d) (g, l').
+
+
+  Inductive Knows (l:local_memory datum) : tid * tid -> Prop :=
+  | knows_def:
+    forall n x y,
+    Node.MapsTo x n (fst cg) ->
+    Locals.MapsTo n (d_task y) l ->
+    Knows l (x, y).
 
 End Defs.
 
-Module Lang.
 
-  Definition to_lang_op (o:op) : Lang.op :=
-  match o with
-(*  | LOCAL_REM _ => Lang.TAU*)
-  | GLOBAL_CREATE x _ => Lang.WRITE x
-  | GLOBAL_PUT x _ => Lang.WRITE x
-  | GLOBAL_GET x => Lang.READ x
-  | FUTURE x _ => Lang.FUTURE x
-  | FORCE x _ => Lang.FORCE x
-  end.
+Section SR.
+  Require SJ_CG.
 
-  Definition to_lang_effects : list effect -> list Lang.effect := List.map (fun (e:effect) => (fst e, to_lang_op (snd e))).
+  Definition LocalToKnows (l:Locals.local_memory datum) cg sj :=
+    forall l p,
+    Knows cg l p ->
+    SJ_CG.Knows (fst cg) sj p.
 
-End Lang.
+  Lemma local_to_knows_reduces:
+    forall a t cg k,
+    Events.Reduces k e k' ->
+    CG.Reduces cg e cg' ->
+    SJ cg k sj ->
+    
+
+End SR.
