src/Shadow.v
@@ -5,7 +5,7 @@ Require Import HJ.Mid.
 Require Import HJ.Cid.
 Require Import HJ.Var.
 Require Import HJ.Dep.
-(*Require Import Node.*)
+Require Import Node.
 
 (* ----- end of boiler-plate code ---- *)
 
@@ -19,264 +19,143 @@ Require Import Coq.Structures.OrderedTypeEx.
 
 Require CG.
 
-Module Trace.
-
+Section Defs.
   (** There are two kinds of events we observe: reading and writing to shared memory. *)
 
-  Inductive mode := READ | WRITE.
+  Variable A:Type.
 
   (**
     An represents the kind of access the node in the CG responsible for the access
     and the target variable.
    *)
 
+  Inductive op := READ | WRITE : A -> op | ALLOC : A -> op.
+
   Structure access := {
-    a_t : mode;           (* how *)
-    a_src : nat; (* when *)
-    a_dst : mid           (* what *)
+    a_when : node;
+    a_what : op
   }.
 
-  Definition access_history := list access.
+Notation WR n x := {| a_when := n; a_what := WRITE x|}.
+Notation RD n := {| a_when := n; a_what := READ|}.
+Notation AL n x := {| a_when := n; a_what := ALLOC x|}.
 
-End Trace.
+  Inductive IsRead a : Prop :=
+  | read_def:
+    a_what a = READ ->
+    IsRead a.
 
-Section Shadow_Ext.
-  Import Trace.
+  Inductive Write a (x:A) : Prop :=
+  | write_write:
+    a_what a = WRITE x ->
+    Write a x
+  | write_alloc:
+    a_what a = ALLOC x ->
+    Write a x.
 
-  (** An access history is just a sequence of optional accesses; none when 
-    the event is neither a read nor a write. *)
+  Inductive IsWrite a : Prop :=
+  | write_def:
+    forall x,
+    Write a x ->
+    IsWrite a.
 
-  (** compares if two access modes. *)
-
-  Definition mode_eq m1 m2 :=
-  match (m1, m2) with
-  | (READ, READ) => true
-  | (WRITE, WRITE) => true
-  | _ => false
-  end.
-
-  (** Matches what and how *)
-
-  Definition a_match x m (a:access) :=
-  andb (Mid.eqb x (a_dst a)) (mode_eq m (a_t a)).
-
-  (** Returns any access that matches what and how. *)
-
-  Definition ah_filter (x:mid) (m:mode) (ah:access_history) := filter (a_match x m) ah.
-
-  (** Returns all reads on a certain variable. *)
-
-  Definition ah_reads (x:mid) (ah:access_history) := ah_filter x READ ah.
-
-  (** Returns all writes on a certain variable *)
-
-  Definition ah_writes x ah := ah_filter x READ ah.
-
-  Section Defs.
-
-  Inductive LastWrite cg ah (a:access) (m:mid) : Prop :=
-  | last_write_def:
-    a_t a = WRITE ->
-    a_dst a = m ->
-    (forall a', a_t a' = WRITE -> List.In (Some a') ah -> CG.HB cg (a_src a') (a_src a)) ->
-    LastWrite cg ah a m.
+  Definition access_history := MM.t (list access).
 
   (** Two accesses are racy *)
 
   Inductive RacyAccess cg : access -> access -> Prop :=
   | racy_access_def:
     forall a b,
-    a_src a <> a_src b ->
-    a_dst a = a_dst b ->
-    (a_t a = WRITE \/ a_t b = WRITE) ->
-    CG.MHP cg (a_src a) (a_src b) ->
+    a_when a <> a_when b ->
+    (IsWrite a \/ IsWrite b) ->
+    CG.MHP cg (a_when a) (a_when b) ->
     RacyAccess cg a b.
-
-  (** Two accesses are race-free. *)
 
   Definition RaceFreeAccess cg a b := ~ RacyAccess cg a b.
 
-  (** An access can be appended to the access-history, yielding a race-free history. *)
-
   Definition RaceFreeCons cg ah a  := Forall (RaceFreeAccess cg a) ah.
 
-  Variable cg:CG.computation_graph.
+Section History.
+
+  Require Import CG.
+
+  Inductive Reduces (cg:computation_graph) ah: (mid * access) -> access_history -> Prop :=
+  | reduces_write:
+    forall n x y l,
+    MM.MapsTo x l ah ->
+    Reduces cg ah (x, WR n y) (MM.add x (WR n y::l) ah)
+  | reduces_read:
+    forall n x l,
+    MM.MapsTo x l ah ->
+    Reduces cg ah (x, {|a_when:=n;a_what:=READ|}) (MM.add x (RD n::l) ah)
+  | reduces_alloc:
+    forall x n y,
+    ~ MM.In x ah ->
+    Reduces cg ah (x, AL n y) (MM.add x (AL n y::nil) ah).
+
+  Section Access.
+
+    Variable h:mid.
+
+    Inductive Access (a:access) (ah:access_history) : Prop :=
+    | access_def:
+      forall l,
+      MM.MapsTo h l ah ->
+      List.In a l ->
+      Access a ah.
+
+    Let Le cg (a:access) b := a = b \/ CG.HB cg (a_when a) (a_when b).
+
+    Inductive LastWrite (n:node) (x:A) ah cg : Prop :=
+    | last_write_def:
+      forall (a:access),
+      Access a ah ->
+      a_when a = n ->
+      Write a x ->
+      (forall b, Access b ah -> IsWrite b -> Le cg b a) ->
+      LastWrite n x ah cg.
+
+    Inductive MapsTo (x:A) ah cg : Prop :=
+    | maps_to_def:
+      forall n,
+      LastWrite n x ah cg ->
+      MapsTo x ah cg.
+
+    Inductive HasRace ah cg : Prop :=
+    | has_race_def:
+      forall a b,
+      Access a ah ->
+      Access b ah ->
+      (IsWrite a \/ IsWrite b) ->
+      CG.MHP cg (a_when a) (a_when b) ->
+      HasRace ah cg.
+
+    Inductive RaceFreeRef ah cg: Prop :=
+    | race_free_ref_def:
+      (forall x y,
+        Access x ah ->
+        Access y ah ->
+        IsWrite y ->
+        x <> y ->
+        CG.Comparable cg (a_when x) (a_when y)) ->
+      RaceFreeRef ah cg.
+  End Access.
 
   Variable ah:access_history.
 
-  Definition Access a t h := List.In {| a_t:=a; a_src:=t; a_dst:=h|} ah. 
-
-  Definition Writes t h := Access WRITE t h.
-
-  Definition Reads t h := Access READ t h.
-
-  Inductive CoAccess (x y:nat) (h:mid): Prop :=
-  | co_access_def:
-    forall a,
-    Writes x h ->
-    Access a y h ->
-    CoAccess x y h.
-
-  Inductive HasRace h : Prop :=
-  | has_race_def:
-    forall n1 n2,
-    CoAccess n1 n2 h ->
-    CG.MHP cg n1 n2 ->
-    HasRace h.
-
-  Inductive RaceFreeRef h: Prop :=
-  | race_free_ref_def:
-    (forall x a y,
-      Access a x h ->
-      Writes y h ->
-      x <> y ->
-      CG.Comparable cg x y) ->
-    RaceFreeRef h.
+  Variable cg:CG.computation_graph.
 
   Inductive RaceFree : Prop :=
   | race_free_def:
-    (forall h, RaceFreeRef h) ->
+    (forall h, RaceFreeRef h ah cg) ->
     RaceFree.
 
   Inductive Racy : Prop :=
     racy_def:
       forall h,
-      HasRace h ->
+      HasRace h ah cg ->
       Racy.
-  End Defs.
+  End History.
 
-  Let race_free_inv_1:
-    forall cg x y t1 t2 h,
-    RaceFreeAccess cg
-      {| a_t := t1; a_src := x; a_dst := h |}
-      {| a_t := t2; a_src := y; a_dst := h |} ->
-    x <> y ->
-    (t1 = WRITE \/ t2 = WRITE) ->
-    CG.Comparable cg x y.
-  Proof.
-    unfold RaceFreeAccess.
-    intros.
-    destruct (CG.hb_dec cg x y).
-    - auto using CG.comparable_left_right.
-    - auto using CG.comparable_right_left.
-    - contradiction.
-    - contradiction H.
-      auto using racy_access_def.
-  Qed.
+End Defs.
 
-  Let race_free_ref_to_race_free_access:
-    forall n1 n2 t1 t2 h cg ah,
-    RaceFreeRef cg ah h ->
-    In {| a_t := t1; a_src := n1; a_dst := h |} ah ->
-    In {| a_t := t2; a_src := n2; a_dst := h |} ah ->
-    RaceFreeAccess cg
-      {| a_t := t1; a_src := n1; a_dst := h |}
-      {| a_t := t2; a_src := n2; a_dst := h |}.
-  Proof.
-    intros.
-    inversion H.
-    unfold RaceFreeAccess.
-    unfold not; intros.
-    inversion H3; simpl in *; subst; clear H5.
-    destruct H6; subst; assert (CG.Comparable cg n1 n2) by eauto using CG.comparable_symm;
-    apply CG.comparable_to_not_mhp in H5; contradiction.
-  Qed.
-
-  Let race_free_access_ref_neq:
-    forall t1 t2 n1 n2 h1 h2 cg,
-    h1 <> h2 ->
-    RaceFreeAccess cg
-       {| a_t := t1; a_src := n1; a_dst := h1 |}
-       {| a_t := t2; a_src := n2; a_dst := h2 |}.
-  Proof.
-    intros.
-    unfold RaceFreeAccess; intuition.
-    inversion H0; simpl in *; subst.
-    contradiction H; auto.
-  Qed.
-
-  Let race_free_to_race_free_access:
-    forall ah cg a1 a2,
-    RaceFree cg ah ->
-    In a1 ah ->
-    In a2 ah ->
-    RaceFreeAccess cg a1 a2.
-  Proof.
-    intros.
-    inversion H.
-    destruct a1, a2; auto.
-    destruct (MID.eq_dec a_dst0 a_dst1); rewrite mid_eq_rw in *; auto.
-    subst.
-    eauto.
-  Qed.
-
-  Lemma race_free_cons:
-    forall cg ah a,
-    RaceFree cg ah ->
-    RaceFreeCons cg ah a ->
-    RaceFree cg (a::ah).
-  Proof.
-    intros.
-    apply race_free_def.
-    intros.
-    apply race_free_ref_def.
-    intros.
-    unfold RaceFreeCons in *.
-    destruct H1.
-    - subst.
-      inversion H2; clear H2.
-      + inversion H1; subst; clear H1.
-        contradiction H3; auto.
-      + rewrite Forall_forall in *.
-        apply H0 in H1.
-        apply race_free_inv_1 in H1; auto.
-    - inversion H2; clear H2.
-      + subst.
-        rewrite Forall_forall in *.
-        apply H0 in H1.
-        apply race_free_inv_1 in H1; auto using CG.comparable_symm.
-      + assert (X: RaceFreeAccess cg
-           {| a_t := a0; a_src := x; a_dst := h |}
-           {| a_t := WRITE; a_src := y; a_dst := h |}) by eauto.
-        apply race_free_inv_1 in X; auto.
-  Qed.
-
-End Shadow_Ext.
-(*
-Module Lang.
-  Import Trace.
-
-  (** Checks if a language event is either a read or a write. *)
-
-  Definition is_access (o:Lang.op) :=
-  match o with
-  | Lang.WRITE _ => true
-  | Lang.READ _ => true
-  | _ => false
-  end.
-
-  (**
-    Converts an event from the language to an event we can interpret.
-    *)
-
-  Definition e_to_a cg (e:Lang.effect) : option access :=
-  match e with
-  | (t, Lang.WRITE m) =>
-    match CG.cg_lookup t cg with
-    | Some n => Some {| a_t:= WRITE; a_src:=n; a_dst:= m |}
-    | _ => None
-    end
-  | (t, Lang.READ m) =>
-    match CG.cg_lookup t cg with
-    | Some n => Some {| a_t:= READ; a_src:=n; a_dst:= m |}
-    | _ => None
-    end
-  | _ => None
-  end.
-
-  Definition effects_to_ah_0 cg : list Lang.effect -> access_history := List.omap (e_to_a cg).
-
-  Definition ah_add cg e ah := e_to_a cg e::ah.
-End Lang.
-
-*)
